# ST95 (Story-Titze 1995) Vocal Fold Model
## Equations of Motion

$$
\begin{align}
F_u &= m_u \ddot{x}_u = F_{ku} + F_{du} - F_{kc} + F_{eu} + F_{uCol} \\
F_l &= m_l \ddot{x}_l = F_{kl} + F_{dl} + F_{kc} + F_{el} + F_{lCol} \\
F_b &= m_b \ddot{x}_b = F_{kb} + F_{db} - [F_{ku} + F_{du} + F_{kl} + F_{dl}] \\
\end{align}
$$

* $\mathbf{M} \triangleq diag(m_u, m_l, m_b)$ - masses
* $\mathbf{x} \triangleq [x_u, x_l, x_b]^T$ - displacements
* $\mathbf{f}_k \triangleq [F_{ku}, F_{kl}, F_{kb}, F_{kc}]^T$ - forces due to spring forces ($F_{kc}$ - spring force due to the coupling of $m_u$ and $m_l$)
* $\mathbf{f}_d \triangleq [F_{du}, F_{dl}, F_{db}]^T$ - forces due to damping
* $\mathbf{f}_{e} \triangleq [F_{eu}, F_{el}, 0]^T$ - external forces generated by the glottal flow
* $\mathbf{f}_{col}\triangleq [F_{uCol}, F_{lCol}, 0]^T$ - forces generated only during collision with the opposite vocal fold

$$
\begin{align}
\mathbf{M} \ddot{\mathbf{x}} &= \begin{bmatrix}1&0&0&-1\\0&1&0&1\\-1&-1&1&0\end{bmatrix} \mathbf{f}_k + \begin{bmatrix}1&0&0\\0&1&0\\-1&-1&1\end{bmatrix} \mathbf{f}_d + \mathbf{f}_{e} + \mathbf{f}_{col}\\
\ddot{\mathbf{x}} &= \mathbf{M}^{-1} \begin{bmatrix}1&0&0&-1\\0&1&0&1\\-1&-1&1&0\end{bmatrix} \mathbf{f}_k + \mathbf{M}^{-1} \begin{bmatrix}1&0&0\\0&1&0\\-1&-1&1\end{bmatrix} \mathbf{f}_d + \mathbf{M}^{-1} \mathbf{f}_{e} + \mathbf{M}^{-1} \mathbf{f}_{col}\\
\end{align}
$$

$$
\begin{align}
F_{ku} &= -k_u [\{( x_u - x_{u0}) - (x_b - x_{b0})\} + \eta_u\{(x_u - x_{u0}) - (x_b - x_{b0})\}^3]\\
F_{kl} &= -k_l [\{( x_l - x_{l0}) - (x_b - x_{b0})\} + \eta_l\{(x_l - x_{l0}) - (x_b - x_{b0})\}^3]\\
F_{kb} &= -k_b[(x_b-x_{b0}) + \eta_b(x_b-x_{b0})^3]
\end{align}
$$

$$
F_{kc} = -k_c [(x_l-x_{l0})-(x_u-x_{u0})]
$$

* Let $\mathbf{y} \triangleq \begin{bmatrix}1 & 0 & -1 \\ 0&1&-1\\0&0&1\end{bmatrix} (\mathbf{x}-\mathbf{x}_0)$


$$
\mathbf{f}_{k} =  -\mathbf{K} \begin{bmatrix}1 & 0 & -1 \\ 0&1&-1\\0&0&1\\-1&1&0\end{bmatrix} (\mathbf{x}-\mathbf{x_0}) -\mathbf{K}\begin{bmatrix}\eta_u&0&0\\0&\eta_l&0\\0&0&\eta_b\end{bmatrix} \mathbf{y}^{\circ3}
$$

* $\mathbf{x}_0 \triangleq [x_u, x_l, x_b]^T$ - equilibrium displacements
* $\mathbf{K} \triangleq \begin{bmatrix}k_u&0&0&k_c\\ 0&k_l&0&k_c\\ 0&0& k_b& 0\end{bmatrix}$ - spring constants


$$
\begin{align}
F_{uCol} &= -h_{uCol} [(x_u-x_{uCol})+\eta_u(x_u-x_{uCol})^3]\\
F_{lCol} &= -h_{lCol} [(x_l-x_{lCol})+\eta_l(x_l-x_{lCol})^3]\\
\end{align}
$$

$$
\mathbf{f}_{col} = -\begin{bmatrix}h_{uCol}&0&0\\0&h_{lCol}&0\\0&0&0\end{bmatrix} \left[ (\mathbf{x}-\mathbf{x_{col}}) + \begin{bmatrix}\eta_u&0&0\\0&\eta_l&0\\0&0&0\end{bmatrix} \left\{ (\mathbf{x}-\mathbf{x_{col}}) \right\} ^{\circ3}\right]
$$

$$
\begin{align}
F_{du} &= -d_u(\dot{x}_u-\dot{x}_b)\\
F_{dl} &= -d_l(\dot{x}_l-\dot{x}_b)\\
F_{db} &= -d_b\dot{x}_b
\end{align}
$$

$$
\begin{align}
d_{l} &= 2\xi_l(m_l k_l)^{1/2}\\
d_{u} &= 2\xi_u(m_u k_u)^{1/2}\\
d_{b} &= 2\xi_b(m_b k_b)^{1/2}
\end{align}
$$

$$
\mathbf{f}_{d} = -\mathbf{D} \begin{bmatrix}1 & 0 & -1 \\ 0&1&-1\\0&0&1\end{bmatrix} \dot{\mathbf{x}}
$$

* $\mathbf{D} \triangleq \begin{bmatrix}d_u&0&0\\0&d_l&0\\0&0&d_b\end{bmatrix}$

-----

$\bm{\theta} = [\mathbf{x}^T | \dot{\mathbf{x}}^T]^T$

$$
\dot{\bm{\theta}} = \begin{bmatrix}
\mathbf{0} & \mathbf{I} \\
\cdot & \cdot
\end{bmatrix} \bm{\theta} + []
$$

$\xi \zeta$
